proof/invariant-abstract/Finalise_AI.thy
@@ -130,7 +130,8 @@ locale Finalise_AI_1 =
           \<and> (cap_irqs cap \<noteq> {} \<longrightarrow> if_unsafe_then_cap s \<and> valid_global_refs s)
           \<and> (is_arch_cap cap \<longrightarrow> pspace_aligned s \<and>
                                  valid_vspace_objs s \<and>
-                                 valid_arch_state s)\<rbrace>
+                                 valid_arch_state s \<and>
+                                 valid_arch_caps s)\<rbrace>
        finalise_cap cap x
      \<lbrace>\<lambda>rv s. replaceable s sl (fst rv) cap\<rbrace>"
   assumes deleting_irq_handler_cte_preserved:
